Safe erasure correctness proof

erasure/theories/SafeErasureFunction.v
@@ -36,6 +36,8 @@ Local Existing Instance extraction_checker_flags.
 Variable Σ : global_env_ext.
 Variable HΣ : ∥wf Σ∥.
 
+Derive Signature for on_global_env.
+
 Definition term_rel : Relation_Definitions.relation (∑ Γ t, wellformed Σ Γ t) :=
   fun '(Γ2; B; H) '(Γ1; t1; H2) =>
     ∥∑ na A, red (fst Σ) Γ1 t1 (tProd na A B) × (Γ1,, vass na A) = Γ2∥.
@@ -415,6 +417,15 @@ Section Erase.
     induction 2; simpl in H => //.
     destruct H as [-> | H].
     constructor. now exists y.
+    now eapply IHX.
+  Qed.
+  
+  Lemma All2_In_right {A B} (P : A -> B -> Type) l l' x' : In x' l' -> 
+    All2 P l l' -> ∥ ∑ x, P x x' ∥.
+  Proof.
+    induction 2; simpl in H => //.
+    destruct H as [-> | H].
+    constructor. now exists x.
     now eapply IHX.
   Qed.
   
@@ -934,8 +945,8 @@ Eval compute in KernameOT.compare (MPfile ["fdejrkjl"], "A") (MPfile ["lfrk;k"],
 
   
 Module KernameSet := MSetList.Make KernameOT.
-(* Module KernameSetFact := WFactsOn Kername KernameSet.
-Module KernameSetProp := WPropertiesOn Kername KernameSet. *)
+(*Module KernameSetFact := WFactsOn Kername KernameSet.
+Module KernameSetProp := WPropertiesOn Kername KernameSet.*)
   
 Fixpoint term_global_deps (t : EAst.term) :=
   match t with
@@ -944,15 +955,20 @@ Fixpoint term_global_deps (t : EAst.term) :=
   | EAst.tLambda _ x => term_global_deps x
   | EAst.tApp x y
   | EAst.tLetIn _ x y => KernameSet.union (term_global_deps x) (term_global_deps y)
-  | EAst.tCase ({| inductive_mind := kn |}, _) x brs =>
-    KernameSet.union (KernameSet.singleton kn) 
+  | EAst.tCase (ind, _) x brs =>
+    KernameSet.union (KernameSet.singleton (inductive_mind ind)) 
       (List.fold_left (fun acc x => KernameSet.union (term_global_deps (snd x)) acc) brs 
         (term_global_deps x))
    | EAst.tFix mfix _ | EAst.tCoFix mfix _ =>
      List.fold_left (fun acc x => KernameSet.union (term_global_deps (EAst.dbody x)) acc) mfix
       KernameSet.empty
+  | EAst.tProj p c => 
+    KernameSet.union (KernameSet.singleton (inductive_mind (fst (fst p))))
+      (term_global_deps c)
   | _ => KernameSet.empty
   end.
+
+
 
 Program Definition erase_constant_body Σ wfΣ (cb : constant_body)
   (Hcb : ∥ on_constant_decl (lift_typing typing) Σ cb ∥) : E.constant_body * KernameSet.t :=  
@@ -971,8 +987,8 @@ Qed.
 
 Definition erase_one_inductive_body (oib : one_inductive_body) : E.one_inductive_body :=
   (* Projection and constructor types are types, hence always erased *)
-  let ctors := map (A:=(ident * term) * nat) (fun '((x, y), z) => (x, EAst.tBox, z)) oib.(ind_ctors) in
-  let projs := map (fun '(x, y) => (x, EAst.tBox)) oib.(ind_projs) in
+  let ctors := map (A:=(ident * term) * nat) (fun '((x, y), z) => (x, z)) oib.(ind_ctors) in
+  let projs := map (fun '(x, y) => x) oib.(ind_projs) in
   {| E.ind_name := oib.(ind_name);
      E.ind_kelim := oib.(ind_kelim);
      E.ind_ctors := ctors;
@@ -1007,80 +1023,514 @@ Next Obligation.
   sq. split. cbn.
   eapply PCUICWeakeningEnv.wf_extends. eauto. eexists [_]; reflexivity.
   now inversion X; subst.
-Defined.
+Qed.
+
 Next Obligation.
   sq.
   inv X. apply X1.
 Qed.
 Next Obligation.
   sq. inv X. apply X0.
-Qed.
+Defined.
 
 Next Obligation.
-  sq. eapply PCUICWeakeningEnv.wf_extends. eauto. eexists [_]; reflexivity.
-Qed.
+  sq. abstract (eapply PCUICWeakeningEnv.wf_extends; eauto; eexists [_]; reflexivity).
+Defined.
 Next Obligation.
-  sq. eapply PCUICWeakeningEnv.wf_extends. eauto. eexists [_]; reflexivity.
-Qed.
+  sq. abstract (eapply PCUICWeakeningEnv.wf_extends; eauto; eexists [_]; reflexivity).
+Defined.
 Next Obligation.
-  sq. eapply PCUICWeakeningEnv.wf_extends. eauto. eexists [_]; reflexivity.
-Qed.
+  sq. abstract (eapply PCUICWeakeningEnv.wf_extends; eauto; eexists [_]; reflexivity).
+Defined.
 
 Program Definition erase_global deps Σ : ∥wf Σ∥ -> _:=
   fun wfΣ  => erase_global_decls deps Σ wfΣ.
 
-Lemma erase_global_correct deps Σ (wfΣ : ∥ wf Σ∥) :
-  erases_global Σ (erase_global deps Σ wfΣ).
+From MetaCoq.Erasure Require Import EDeps.
+Lemma lookup_env_nil c s : lookup_env [] c = Some s -> False.
 Proof.
-  induction Σ in wfΣ |- *; intros; sq.
-  - simpl. constructor.
-  - destruct a as [kn [|]]; simpl.
-    destruct KernameSet.mem => //.
-(*
+  induction c; simpl; auto => //.
+Qed.
+
+Definition global_erased_with_deps Σ Σ' kn :=
+  (exists cst, declared_constant Σ kn cst /\
+   exists cst' : EAst.constant_body,
+    ETyping.declared_constant Σ' kn cst' /\
+    erases_constant_body (Σ, cst_universes cst) cst cst' /\
+    (forall body : EAst.term,
+     EAst.cst_body cst' = Some body -> erases_deps Σ Σ' body)) \/
+  (exists mib, declared_minductive Σ kn mib).
+
+Definition includes_deps Σ Σ' deps :=  
+  forall kn, 
+    KernameSet.In kn deps ->
+    global_erased_with_deps Σ Σ' kn.
+
+Lemma includes_deps_union Σ Σ' deps deps' :
+  includes_deps Σ Σ' (KernameSet.union deps deps') ->
+  includes_deps Σ Σ' deps /\ includes_deps Σ Σ' deps'.
+Proof.
+  intros.
+  split; intros kn knin; eapply H; rewrite KernameSet.union_spec; eauto.
+Qed.
+
+Lemma in_fold_left {A} kn f (l : list A) acc : 
+  KernameSet.In kn (fold_left (fun acc x => KernameSet.union (f x) acc) l acc) <->
+  (KernameSet.In kn acc \/ exists a, In a l /\ KernameSet.In kn (f a)).
+Proof.
+  induction l in acc |- *; simpl. intuition auto.
+  now destruct H0.
+  rewrite IHl. rewrite KernameSet.union_spec.
+  intuition auto.
+  right. now exists a.
+  destruct H0 as [a' [ina inkn]].
+  right. now exists a'.
+  destruct H0 as [a' [ina inkn]].
+  destruct ina as [<-|ina'];
+  intuition auto. right. now exists a'.
+Qed.
+
+Lemma includes_deps_fold {A} Σ Σ' brs deps (f : A -> EAst.term) :
+  includes_deps Σ Σ'
+  (fold_left
+    (fun (acc : KernameSet.t) (x : A) =>
+      KernameSet.union (term_global_deps (f x)) acc) brs
+      deps) ->
+  includes_deps Σ Σ' deps /\
+  (forall x, In x brs ->
+    includes_deps Σ Σ' (term_global_deps (f x))).
+Proof.
+  intros incl; split.
+  intros kn knin; apply incl.
+  rewrite in_fold_left. left; auto.
+  intros br brin. intros kn knin. apply incl.
+  rewrite in_fold_left. right.
+  now exists br.
+Qed.
+
+Lemma In_Forall {A} {P : A -> Prop} l : 
+  (forall x, In x l -> P x) ->
+  Forall P l.
+Proof.
+  intros H; induction l; constructor; auto.
+  now apply H; simpl. apply IHl.
+  intros x xin; apply H; simpl; auto.
+Qed.
+
+Lemma Forall2_All2 {A B} {P : A -> B -> Prop} l l' : Forall2 P l l' -> All2 P l l'.
+Proof.
+  intros f; induction l in l', f |- *; destruct l'; try constructor; auto.
+  elimtype False. inv f.
+  elimtype False. inv f.
+  inv f; auto.
+  apply IHl. inv f; auto.
+Qed.
+
+Definition declared_kn Σ kn :=
+  ∥ ∑ decl, lookup_env Σ kn = Some decl ∥.
+
+Lemma term_global_deps_spec {cf:checker_flags} {Σ Γ t et T} : 
+  wf Σ.1 ->
+  Σ ;;; Γ |- t : T ->
+  Σ;;; Γ |- t ⇝ℇ et ->
+  forall x, KernameSet.In x (term_global_deps et) -> declared_kn Σ.1 x.
+Proof.
+  intros wf wt er.
+  induction er in T, wt |- * using erases_forall_list_ind;
+    cbn in *; try solve [constructor]; intros kn' hin;
+    repeat match goal with 
+    | [ H : KernameSet.In _ KernameSet.empty |- _ ] =>
+      now apply KernameSet.empty_spec in hin
+    | [ H : KernameSet.In _ (KernameSet.union _ _) |- _ ] =>
+      apply KernameSet.union_spec in hin as [?|?]
+    end.
+  - apply inversion_Lambda in wt as (? & ? & ? & ? & ?); eauto.
+  - apply inversion_LetIn in wt as (? & ? & ? & ? & ? & ?); eauto.
+  - apply inversion_LetIn in wt as (? & ? & ? & ? & ? & ?); eauto.
+  - apply inversion_App in wt as (? & ? & ? & ? & ? & ?); eauto.
+  - apply inversion_App in wt as (? & ? & ? & ? & ? & ?); eauto.
+  - apply inversion_Const in wt as (? & ? & ? & ? & ?); eauto.
+    eapply KernameSet.singleton_spec in hin; subst.
+    red in d. red. sq. rewrite d. intuition eauto.
+  - apply inversion_Construct in wt as (? & ? & ? & ? & ? & ? & ?); eauto.
+    destruct kn.
+    eapply KernameSet.singleton_spec in hin; subst.
+    destruct d as [[H _] _]. red in H. simpl in *.
+    red. sq. rewrite H. intuition eauto.
+  - apply inversion_Case in wt
+      as (? & ? & ? & ? & ? & ? & ? & ? & ? & ? & ? & ? & ? & ? & ? & ? & ?); eauto.
+    destruct ind as [kn i']; simpl in *.
+    eapply KernameSet.singleton_spec in H1; subst.
+    destruct d as [d _]. red in d.
+    simpl in *. eexists; intuition eauto.
+
+  - apply inversion_Case in wt
+    as (? & ? & ? & ? & ? & ? & ? & ? & ? & ? & ? & ? & ? & ? & ? & ? & ?); eauto.
+    eapply in_fold_left in H1.
+    destruct H1. eapply IHer; eauto.
+    destruct H1 as [br [inbr inkn]].
+    eapply Forall2_All2 in H0.
+    assert (All (fun br => ∑ T, Σ ;;; Γ |- br.2 : T) brs).
+    eapply All2_All_left. eapply a.
+    simpl. intuition auto. eexists ; eauto.
+    eapply All2_All_mix_left in H0; eauto. simpl in H0.
+    eapply All2_In_right in H0; eauto.
+    destruct H0.
+    destruct X1 as [br' [[T' HT] ?]].
+    eauto.
+
+  - eapply KernameSet.singleton_spec in H0; subst.
+    apply inversion_Proj in wt as (?&?&?&?&?&?&?&?&?); eauto.
+    destruct d as [[d _] _]. red in d. eexists; eauto.
+
+  - apply inversion_Proj in wt as (?&?&?&?&?&?&?&?&?); eauto.
+
+  - apply inversion_Fix in wt as (?&?&?&?&?&?&?); eauto.
+    eapply in_fold_left in hin as [|].
+    now eapply KernameSet.empty_spec in H0.
+    destruct H0 as [? [ina indeps]].
+    eapply Forall2_All2 in H.
+    eapply All2_All_mix_left in H; eauto.
+    eapply All2_In_right in H; eauto.
+    destruct H as [[def [[Hty _] Hdef]]].
+    eapply Hdef; eauto.
+
+  - apply inversion_CoFix in wt as (?&?&?&?&?&?&?); eauto.
+    eapply in_fold_left in hin as [|].
+    now eapply KernameSet.empty_spec in H0.
+    destruct H0 as [? [ina indeps]].
+    eapply Forall2_All2 in H.
+    eapply All2_All_mix_left in H; eauto.
+    eapply All2_In_right in H; eauto.
+    destruct H as [[def [Hty Hdef]]].
+    eapply Hdef; eauto.
+Qed.
+
+Lemma erase_global_erases_deps {Σ Σ' t et T} : 
+  wf_ext Σ ->
+  Σ;;; [] |- t : T ->
+  Σ;;; [] |- t ⇝ℇ et ->
+  includes_deps Σ Σ' (term_global_deps et) ->
+  erases_deps Σ Σ' et.
+Proof.
+  intros wf wt er.
+  induction er in er, t, T, wf, wt |- * using erases_forall_list_ind;
+    cbn in *; try solve [constructor]; intros Σer;
+    repeat match goal with 
+    | [ H : includes_deps _ _ (KernameSet.union _ _ ) |- _ ] =>
+      apply includes_deps_union in H as [? ?]
+    end.
+  - now apply inversion_Evar in wt.
+  - constructor.
+    now apply inversion_Lambda in wt as (? & ? & ? & ? & ?); eauto.
+  - apply inversion_LetIn in wt as (? & ? & ? & ? & ? & ?); eauto.
+    constructor; eauto.
+  - apply inversion_App in wt as (? & ? & ? & ? & ? & ?); eauto.
+    now constructor; eauto.
+  - apply inversion_Const in wt as (? & ? & ? & ? & ?); eauto.
+    specialize (Σer kn).
+    forward Σer. rewrite KernameSet.singleton_spec //.
+    destruct Σer as [[c' [declc' (? & ? & ? & ?)]]|].
+    pose proof (PCUICWeakeningEnv.declared_constant_inj _ _ d declc'). subst x.
+    now econstructor; eauto.
+    destruct H as [mib declm].
+    red in declm, d. rewrite d in declm. noconf declm.
+  - apply inversion_Case in wt
+      as (? & ? & ? & ? & ? & ? & ? & ? & ? & ? & ? & ? & ? & ? & ? & ? & ?); eauto.
+    destruct ind as [kn i']; simpl in *.
+    apply includes_deps_fold in H2 as [? ?].
+    eapply erases_deps_tCase; eauto.
+    eapply In_Forall in H3.
+    eapply All_Forall. eapply Forall_All in H3.
+    eapply Forall2_All2 in H0.
+    eapply All2_All_mix_right in H0; eauto.
+    assert (All (fun br => ∑ T, Σ ;;; Γ |- br.2 : T) brs).
+    eapply All2_All_left. eapply a.
+    simpl. intuition auto. eexists ; eauto.
+    ELiftSubst.solve_all. destruct a2 as [T' HT]. eauto.
+
+  - apply inversion_Proj in wt as (?&?&?&?&?&?&?&?&?); eauto.
     constructor.
-    + simpl.
-      destruct c as [na [b|] ty]; simpl.
-      apply erases_erase. constructor.  
-    + apply IHΣ.
-    + red. simpl.
-      eapply (erases_global_ind _ (ind_universes m)).
-      inv w. red in X0.
-      destruct m; simpl; intuition; try constructor. all:simpl; auto.
-      eapply All2_Forall2.
-      eapply All2_from_nth_error.
-      now autorewrite with len.
-      intros.
-      rewrite nth_error_map H0 /= in H2. noconf H2.
-     red. simpl.
-      destruct X0; simpl in *.
-      eapply Alli_nth_error in onInductives; eauto.
-      destruct onInductives. rewrite ind_arity_eq /=.
-      rewrite decompose_prod_n_assum_it_mkProd /=.
-      intuition auto.
-      rewrite -{1}(map_id (ind_ctors x1)).
-      eapply Forall2_map.
-      eapply All2_Forall2.
-      red in onConstructors.
-      eapply All2_from_nth_error; auto. intros.
-      rewrite H4 in H5; noconf H5.
-      eapply All2_nth_error_Some in onConstructors; eauto.
-      destruct onConstructors as [cshape [Hnth onc]].
-      destruct onc ; simpl in *.
-      destruct x0 as [[id ty] nargs]; intuition auto.
-      constructor. eapply isType_isErasable.
-      simpl in on_ctype. red in on_ctype. eapply on_ctype.
-      rewrite -{1}(map_id (ind_projs x1)).
-      eapply All2_Forall2. eapply All2_map.
-      eapply All2_from_nth_error; auto. intros.
-      rewrite H4 in H5; noconf H5.
-      forward onProjections.
-      destruct (ind_projs x1); simpl in *; try congruence. lia.
-      destruct ind_cshapes; simpl in *.
-      destruct onProjections. destruct ind_cshapes => //.
-      destruct x0 as [id ty]. intuition auto.
-      constructor.
-      eapply isType_isErasable.
-      todo "erasure of projection types".
-      apply IHΣ.
-      *)
-Admitted.
+    now eapply IHer; eauto.
+  - constructor.
+    apply inversion_Fix in wt as (?&?&?&?&?&?&?); eauto.
+    eapply All_Forall. eapply includes_deps_fold in Σer as [_ Σer].
+    eapply In_Forall in Σer.
+    eapply Forall_All in Σer.
+    eapply Forall2_All2 in H.
+    ELiftSubst.solve_all.
+  - constructor.
+    apply inversion_CoFix in wt as (?&?&?&?&?&?&?); eauto.
+    eapply All_Forall. eapply includes_deps_fold in Σer as [_ Σer].
+    eapply In_Forall in Σer.
+    eapply Forall_All in Σer.
+    eapply Forall2_All2 in H.
+    ELiftSubst.solve_all.
+Qed.
+
+From MetaCoq.PCUIC Require Import PCUICReflect PCUICWeakeningEnv.
+Lemma lookup_env_cons {kn d Σ kn' d'} : lookup_env ((kn, d) :: Σ) kn' = Some d' ->
+  (kn = kn' /\ d = d') \/ (kn <> kn' /\ lookup_env Σ kn' = Some d').
+Proof.
+  simpl.
+  epose proof (eqb_spec (A:=kername) kn' kn). simpl in H.
+  elim: H. intros -> [= <-]; intuition auto.
+  intros diff look. intuition auto.
+Qed.
+
+Lemma lookup_env_cons_fresh {kn d Σ kn'} : 
+  kn <> kn' ->
+  lookup_env ((kn, d) :: Σ) kn' = lookup_env Σ kn'.
+Proof.
+  simpl.
+  epose proof (eqb_spec (A:=kername) kn' kn). simpl in H.
+  elim: H. intros -> => //. auto.
+Qed.
+
+Lemma elookup_env_cons_fresh {kn d Σ kn'} : 
+  kn <> kn' ->
+  ETyping.lookup_env ((kn, d) :: Σ) kn' = ETyping.lookup_env Σ kn'.
+Proof.
+  simpl. destruct kername_eq_dec. subst => //. auto. 
+Qed.
+
+Lemma erases_weakeninv_env {Σ Σ' : global_env_ext} {Γ t t' T} :
+  wf Σ -> wf Σ' -> extends Σ Σ' -> 
+  Σ ;;; Γ |- t : T ->
+  erases Σ Γ t t' -> erases (Σ'.1, Σ.2) Γ t t'.
+Proof.
+  intros wfΣ wfΣ' ext Hty.
+  apply (env_prop_typing _ _ ESubstitution.erases_extends _ wfΣ _ _ _ Hty _ wfΣ' ext).
+Qed.  
+ 
+Lemma erases_deps_weaken kn d Σ Σ' t : 
+  wf ((kn, d) :: Σ) ->
+  erases_deps Σ Σ' t ->
+  erases_deps ((kn, d) :: Σ) Σ' t.
+Proof.
+  intros wfΣ er.
+  induction er using erases_deps_forall_ind; try solve [now constructor].
+  assert (kn <> kn0).
+  { inv wfΣ. intros <-.
+    eapply lookup_env_Some_fresh in H. contradiction. }
+  eapply erases_deps_tConst with cb cb'; eauto.
+  red. rewrite lookup_env_cons_fresh //.
+  red.
+  red in H1.
+  destruct (cst_body cb) eqn:cbe;
+  destruct (E.cst_body cb') eqn:cbe'; auto.
+  specialize (H3 _ eq_refl).
+  eapply on_declared_constant in H; auto.
+  2:{ now inv wfΣ. }
+  red in H. rewrite cbe in H. simpl in H.
+  eapply (erases_weakeninv_env (Σ := (Σ, cst_universes cb))
+     (Σ' := (((kn, d) :: Σ), cst_universes cb))); eauto.
+  simpl. now inv wfΣ.
+  eexists [(kn, d)]; intuition eauto.
+Qed.
+
+Lemma global_erases_with_deps_cons kn kn' d d' Σ Σ' : 
+  wf ((kn', d) :: Σ) ->
+  global_erased_with_deps Σ Σ' kn ->
+  global_erased_with_deps ((kn', d) :: Σ) ((kn', d') :: Σ') kn.
+Proof.
+  intros wf [[cst [declc [cst' [declc' [ebody IH]]]]]|].
+  red. inv wf. left.
+  exists cst. split.
+  red in declc |- *.
+  rewrite lookup_env_cons_fresh //.
+  { eapply lookup_env_Some_fresh in declc.
+    intros <-; contradiction. }
+  exists cst'.
+  unfold ETyping.declared_constant. rewrite elookup_env_cons_fresh //.
+  { eapply lookup_env_Some_fresh in declc.
+    intros <-; contradiction. }
+  red in ebody. unfold erases_constant_body.
+  destruct (cst_body cst) eqn:bod; destruct (E.cst_body cst') eqn:bod' => //.
+  intuition auto.
+  eapply (erases_weakeninv_env (Σ  := (_, cst_universes cst)) (Σ' := ((kn', d) :: Σ, cst_universes cst))); eauto.
+  constructor; eauto.
+  exists [(kn', d)]; intuition eauto.
+  eapply on_declared_constant in declc; auto.
+  red in declc. rewrite bod in declc. eapply declc.
+  noconf H.
+  eapply erases_deps_cons; eauto.
+  constructor; auto.
+
+  right. destruct H as [mib Hm].
+  exists mib.
+  red.
+  rewrite lookup_env_cons_fresh //.
+  inv wf.
+  { eapply lookup_env_Some_fresh in Hm.
+    intros <-; contradiction. }
+Qed.
+
+Lemma global_erases_with_deps_weaken kn kn' d Σ Σ' : 
+  wf ((kn', d) :: Σ) ->
+  global_erased_with_deps Σ Σ' kn ->
+  global_erased_with_deps ((kn', d) :: Σ) Σ' kn.
+Proof.
+  intros wf [[cst [declc [cst' [declc' [ebody IH]]]]]|].
+  red. inv wf. left.
+  exists cst. split.
+  red in declc |- *.
+  rewrite lookup_env_cons_fresh //.
+  { eapply lookup_env_Some_fresh in declc.
+    intros <-; contradiction. }
+  exists cst'.
+  unfold ETyping.declared_constant.
+  red in ebody. unfold erases_constant_body.
+  destruct (cst_body cst) eqn:bod; destruct (E.cst_body cst') eqn:bod' => //.
+  intuition auto.
+  eapply (erases_weakeninv_env (Σ  := (_, cst_universes cst)) (Σ' := ((kn', d) :: Σ, cst_universes cst))); eauto.
+  constructor; eauto.
+  exists [(kn', d)]; intuition eauto.
+  eapply on_declared_constant in declc; auto.
+  red in declc. rewrite bod in declc. eapply declc.
+  noconf H.
+  eapply erases_deps_weaken; eauto. constructor; eauto.
+
+  right. destruct H as [mib Hm].
+  exists mib.
+  red.
+  rewrite lookup_env_cons_fresh //.
+  inv wf.
+  { eapply lookup_env_Some_fresh in Hm.
+    intros <-; contradiction. }
+Qed.
+
+Lemma erase_constant_body_correct Σ Σ' cb (wfΣ : ∥  wf_ext Σ ∥) (onc : ∥ on_constant_decl (lift_typing typing) Σ cb ∥) :
+  wf Σ' -> extends Σ Σ' ->   
+  erases_constant_body (Σ', Σ.2) cb (fst (erase_constant_body Σ wfΣ cb onc)).
+Proof.
+  red. sq. destruct cb as [name [bod|] univs]; simpl. intros.
+  eapply (erases_weakeninv_env (Σ := Σ) (Σ' := (Σ', univs))); simpl; auto.
+  red in o. simpl in o. eapply o.
+  eapply erases_erase. auto.
+Qed.
+
+Lemma erase_constant_body_correct' {Σ cb} {wfΣ : ∥  wf_ext Σ ∥} {onc : ∥ on_constant_decl (lift_typing typing) Σ cb ∥} {body} :
+  EAst.cst_body (fst (erase_constant_body Σ wfΣ cb onc)) = Some body ->
+  ∥ ∑ t T, (Σ ;;; [] |- t : T) * (Σ ;;; [] |- t ⇝ℇ body) *
+      (term_global_deps body = snd (erase_constant_body Σ wfΣ cb onc)) ∥.
+Proof.
+  intros. destruct cb as [name [bod|] univs]; simpl. intros.
+  simpl in H. noconf H.
+  set (obl :=(erase_constant_body_obligation_1 Σ wfΣ
+  {|
+  PA.cst_type := name;
+  PA.cst_body := Some bod;
+  PA.cst_universes := univs |} onc bod eq_refl)). clearbody obl.
+  destruct obl. sq.
+  exists bod, A; intuition auto. simpl.
+  eapply erases_erase. now simpl in H.
+Qed.
+
+Lemma erase_global_includes Σ deps deps' wfΣ :
+  (forall d, KernameSet.In d deps' -> ∥ ∑ decl, lookup_env Σ d = Some decl ∥) ->
+  KernameSet.subset deps' deps ->
+  includes_deps Σ (erase_global deps Σ wfΣ) deps'.
+Proof.
+  sq.
+  induction Σ in deps, deps', w |- *; simpl; intros H.
+  - intros sub i hin. elimtype False.
+    specialize (H i hin) as [[decl Hdecl]]. noconf Hdecl.
+  - intros sub i hin.
+    destruct a as [kn d].
+    eapply KernameSet.subset_spec in sub.
+    destruct (H i hin) as [[decl Hdecl]].
+    pose proof (eqb_spec i kn). simpl in H0.
+    revert Hdecl; elim: H0. intros -> [= <-].
+    * destruct d as [|]; [left|right].
+      exists c. split; auto.
+      red. simpl. rewrite eq_kername_refl //.
+      pose proof (sub _ hin) as indeps.
+      eapply KernameSet.mem_spec in indeps. rewrite indeps.
+      unfold ETyping.declared_constant. simpl.
+      destruct (kername_eq_dec kn kn); simpl.
+      eexists; intuition eauto.
+      eapply erase_constant_body_correct; eauto.
+      exists [(kn, ConstantDecl c)]; intuition auto.
+      eapply erases_deps_cons; auto.
+      assert (wf Σ). clear H0; now inv w.
+    
+      pose proof (erase_constant_body_correct' H0).
+      sq. destruct X0 as [bod [bodty [[Hbod Hebod] Heqdeps]]].
+      eapply (erase_global_erases_deps (Σ := (Σ, cst_universes c))); simpl; auto.
+      constructor; simpl; auto.
+      depelim w. auto. eauto. eauto.
+      eapply IHΣ.
+
+      intros d ind. todo "non circular".
+      rewrite -Heqdeps. eapply KernameSet.subset_spec.
+      intros x hin'. eapply KernameSet.union_spec. right; auto.
+      congruence.
+      eexists; intuition auto. red.
+      simpl. rewrite eq_kername_refl. reflexivity.
+    * intros ikn Hi.
+      destruct d as [|].
+      ++ destruct (KernameSet.mem kn deps) eqn:eqkn.
+        eapply global_erases_with_deps_cons; eauto.
+        eapply (IHΣ _ (KernameSet.singleton i)); auto.
+        3:{ eapply KernameSet.singleton_spec => //. }
+        intros.
+        eapply KernameSet.singleton_spec in H0. subst.
+        constructor; exists decl; auto.
+        eapply KernameSet.subset_spec. intros ? ?.
+        eapply KernameSet.union_spec. left.
+        eapply KernameSet.singleton_spec in H0; subst.
+        now eapply sub.
+      
+        eapply global_erases_with_deps_weaken. eauto.
+        unfold erase_global_decls_obligation_4. simpl.
+        eapply (IHΣ deps (KernameSet.singleton i)).
+        3:now eapply KernameSet.singleton_spec.
+        intros d ind%KernameSet.singleton_spec.
+        subst. constructor; eexists; eauto.
+        eapply KernameSet.subset_spec.
+        intros ? hin'. eapply sub. eapply KernameSet.singleton_spec in hin'. now subst.        
+
+      ++ destruct (KernameSet.mem kn deps) eqn:eqkn.
+        eapply global_erases_with_deps_cons; eauto.
+        eapply (IHΣ _ (KernameSet.singleton i)); auto.
+        3:{ eapply KernameSet.singleton_spec => //. }
+        intros.
+        eapply KernameSet.singleton_spec in H0. subst.
+        constructor; exists decl; auto.
+        eapply KernameSet.subset_spec. intros ? ?.
+        eapply KernameSet.singleton_spec in H0; subst.
+        now eapply sub.
+    
+        eapply global_erases_with_deps_weaken. eauto.
+        unfold erase_global_decls_obligation_4. simpl.
+        eapply (IHΣ deps (KernameSet.singleton i)).
+        3:now eapply KernameSet.singleton_spec.
+        intros d ind%KernameSet.singleton_spec.
+        subst. constructor; eexists; eauto.
+        eapply KernameSet.subset_spec.
+        intros ? hin'. eapply sub. eapply KernameSet.singleton_spec in hin'. now subst.        
+Qed.
+
+Lemma erase_correct (Σ : global_env_ext) (wfΣ : wf_ext Σ) t T v Σ' t' :
+  axiom_free Σ.1 ->
+  forall wt : Σ ;;; [] |- t : T,
+  erase Σ (sq wfΣ) [] t (iswelltyped wt) = t' ->
+  erase_global (term_global_deps t') Σ (sq (wfΣ.1)) = Σ' ->
+  Σ |-p t ▷ v -> 
+  exists v', Σ;;; [] |- v ⇝ℇ v' /\ ∥Σ' ⊢ t' ▷ v'∥.
+Proof.
+  intros axiomfree wt.
+  generalize (iswelltyped wt).
+  generalize (sq wfΣ.1) as swfΣ.
+  intros swfΣ wt' HΣ' Ht' ev.
+  assert (extraction_pre Σ) by now constructor.
+  pose proof (erases_erase (wfΣ := sq wfΣ) wt'); eauto.
+  rewrite HΣ' in H.
+  unshelve epose proof (erase_global_erases_deps wfΣ wt H _); cycle 2.
+  eapply erases_correct; eauto.
+  rewrite <- Ht'.
+  eapply erase_global_includes.
+  intros. 2:eapply KernameSet.subset_spec; intros ? ?; auto.
+  eapply term_global_deps_spec in H; eauto.
+Qed.
